new/golang/theory.v
@@ -1,9 +1,10 @@
 From Perennial.goose_lang Require Export lang.
 From New.golang Require Export defn.
+(* required just to make sure this demo works *)
+From New.golang.theory Require mem.
 From New.golang.theory Require Export exception list typing dynamic_typing loop struct
   slice map interface defer typing builtin primitive chan pkg auto globals.
-(* note dynamic_mem is last to shadow parts of mem *)
-From New.golang.theory Require Export mem dynamic_mem.
+From New.golang.theory Require Export typed_pointsto dynamic_mem.
 From Perennial Require Export base.
 
 Export uPred. (* XXX: inherited from proof_prelude.v; not sure why it's here. *)
