new/golang/theory/struct.v
@@ -1,9 +1,11 @@
 From Perennial.goose_lang Require Import lifting.
 From New.golang.defn Require Export struct.
-From New.golang.theory Require Import mem exception list typing.
+From New.golang.theory Require Import typed_pointsto exception list typing.
 From Perennial.Helpers Require Import NamedProps.
 From RecordUpdate Require Export RecordUpdate.
 From Perennial Require Import base.
+
+Set Default Proof Using "Type".
 
 Module struct.
 Section goose_lang.
